Modifying abstract syntax, now simpler type system. Implemented Environment.v for design and design state environment definitions. Implemented is_of_type relation in IsOfType (in_c relation). Implemented is_gstatic and is_lstatic in StaticExpressions. Added TypeElaboration.v to implement type elab relation, but we need expr eval relation first. In order to implement expr. eval. relation, started to work on Array module definition based on Vector (list with size).

hvhdl/AbstractSyntax.v
@@ -22,109 +22,90 @@ and | or | eq | neq | lt | le | gt | ge | add | sub.
  *)
 
 Inductive expr : Type :=
-| Enat : nat -> expr (** Natural constant *)
-| Ebool : bool -> expr (** Boolean constant *)
-| Ename : name -> expr (** Name constant *)
-| Eaggreg : list expr -> expr (** Aggregate of expressions *)
-| Ebinop : binop -> expr -> expr -> expr (** Binary operator expression *)
-| Enot : expr -> expr (** Not expression *)
+| e_nat : nat -> expr (** Natural constant *)
+| e_bool : bool -> expr (** Boolean constant *)
+| e_name : name -> expr (** Name constant *)
+| e_arc : arc_t -> expr (** [arc_t] constant *)
+| e_trans : transition_t -> expr (** [transition_t] constant *)
+| e_aggreg : list expr -> expr (** Aggregate of expressions *)
+| e_binop : binop -> expr -> expr -> expr (** Binary operator expression *)
+| e_not : expr -> expr (** Not expression *)
 
 (** Names *)
 with name : Type :=
-| Nid : ident -> name  
-| Nxid : ident -> expr -> name.
+| n_id : ident -> name  
+| n_xid : ident -> expr -> name.
 
 (** Subtype indications and type definitions. *)
 
 Inductive tind : Type :=
-| Tid (id : ident) (** Simple subtype indication. *)
-| Tcid (id : ident) (constr : expr * expr). (** Subtype indication with constraint. *)
-
-Inductive tdef : Type :=
-
-(** Unconstrained array definition. *)
-| Tarray (eltt : tind)
-         
-(** Constrained array definition. *)
-| Tcarray (eltt : tind) (constr : expr * expr)
-          
-(** Type definition as an enumeration of idents with at least one element. 
-    [lme] is the left-most element.
- *)
-| Tenum (lme : ident) (enum : list ident).    
+| tind_boolean                         (** Boolean type indication. *)
+| tind_natural (rconstr : expr * expr) (** Natural with range constraint. *)
+| tind_arc_t                           (** arc_t type indication. *)
+| tind_transition_t                    (** transition_t type indication. *)
+| tind_array (t : tind) (iconstr : expr * expr). (** Array of [t] with index constraint. *)
 
 (** ** Sequential statements. *)
 
 Inductive ss : Type :=
-| Ssig (signame : name) (e : expr)                      (** Signal assignment statement. *)
-| Svar (varname : name) (e : expr)                      (** Variable assignment statement. *)
-| Sif (e : expr) (stmt : ss)                            (** If statement. *)
-| Sifelse (e : expr) (stmt : ss) (stmt' : ss)           (** If then else statement. *)
-| Sloop (id : ident) (e : expr) (e' : expr) (stmt : ss) (** Loop statement. *)
-| Sfalling (stmt : ss)                                  (** Falling edge block statement. *)
-| Srising (stmt : ss)                                   (** Rising edge block statement. *)
-| Sseq (stmt : ss) (stmt' : ss).                        (** Composition of seq. statements. *)
+| ss_sig (signame : name) (e : expr)                      (** Signal assignment statement. *)
+| ss_var (varname : name) (e : expr)                      (** Variable assignment statement. *)
+| ss_if (e : expr) (stmt : ss)                            (** If statement. *)
+| ss_ifelse (e : expr) (stmt : ss) (stmt' : ss)           (** If then else statement. *)
+| ss_loop (id : ident) (e : expr) (e' : expr) (stmt : ss) (** Loop statement. *)
+| ss_falling (stmt : ss)                                  (** Falling edge block statement. *)
+| ss_rising (stmt : ss)                                   (** Rising edge block statement. *)
+| ss_seq (stmt : ss) (stmt' : ss).                        (** Composition of seq. statements. *)
 
-Notation "stmt ;; stmt'" := (Sseq stmt stmt') (at level 100).
+Notation "stmt ;; stmt'" := (ss_seq stmt stmt') (at level 100).
 
 (** ** Concurrent statements. *)
 
 Inductive cs : Type :=
 
 (** Process statement. *)
-| Cps (pid : ident)                (** Process id *)
-      (sl : list ident)            (** Sensitivity list *)
-      (vars : list (ident * tind)) (** Variable declaration list *)
-      (stmt : ss)                  (** Sequential statement block *)
+| cs_ps (pid : ident)                (** Process id *)
+        (sl : list ident)            (** Sensitivity list *)
+        (vars : list (ident * tind)) (** Variable declaration list *)
+        (stmt : ss)                  (** Sequential statement block *)
       
 (** Component instantiation statement. *)
-| Ccomp (compid : ident)                     (** Component id *)
-        (entid : ident)                      (** Entity label *)
-        (gmap : list (ident * expr))         (** Generic map *)
-        (ipmap : list (name * expr))         (** In port map *)
-        (opmap : list (name * option name))  (** Out port map, 'n => None' ≡ 'n => open' *)
+| cs_comp (compid : ident)                     (** Component id *)
+          (entid : ident)                      (** Entity label *)
+          (gmap : list (ident * expr))         (** Generic map *)
+          (ipmap : list (name * expr))         (** In port map *)
+          (opmap : list (name * option name))  (** Out port map, 'n => None' ≡ 'n => open' *)
 
 (** Composition of concurrent statements. *)
-| Cpar (cstmt : cs) (cstmt' : cs).
+| cs_par (cstmt : cs) (cstmt' : cs).
 
-Notation "cstmt // cstmt'" := (Cpar cstmt cstmt') (at level 0).
+Notation "cstmt // cstmt'" := (cs_par cstmt cstmt') (at level 0).
 
 (** ** Design declaration. *)
 
 (** Generic constant declaration. *)
 
 Inductive gdecl : Type :=
-  Gen (genid : ident) (t : tind) (e : expr).
+  gdecl_ (genid : ident) (t : tind) (e : expr).
 
 (** Architecture declarations. *)
 
 Inductive adecl : Type :=
-| Atdef (tid : ident) (t : tdef)                  (** Type definition declaration. *)
-| Atind (tid : ident) (t : tind)                  (** Subtype indication declaration. *)
-| Asig (sigid : ident) (t : tind)                 (** Signal declaration. *)
-| Aconst (constid : ident) (t : tind) (v : expr). (** Constant declaration. *)
+| adecl_sig (sigid : ident) (t : tind)                 (** Signal declaration. *)
+| adecl_const (constid : ident) (t : tind) (v : expr). (** Constant declaration. *)
 
 (** Port declarations. *)
 
 Inductive pdecl : Type :=
-| Pin (portid : ident) (t : tind)
-| Pout (portid : ident) (t : tind).
+| pdecl_in (portid : ident) (t : tind)
+| pdecl_out (portid : ident) (t : tind).
 
 (** Design declaration. *)
 
 Inductive design : Type :=
-  Design (entid : ident)       (** Entity id *)
-         (archid : ident)      (** Architecture id *)
-         (gens : list gdecl)   (** Generic constant list *)
-         (ports : list pdecl)  (** Port list *)
-         (adecls : list adecl) (** Architecture declarative part *)
-         (cstmt : cs).         (** Concurrent statement part *)
-
-Example design0 :=
-  Design 0 1
-         [(Gen 2 (Tid 3) (Enat 2)); (Gen 3 (Tid 3) (Enat 2))]
-         [(Pin 8 (Tid 3)); (Pin 9 (Tcid 3 ((Enat 4), (Enat 9))))]
-         []
-         ((Cps 5 [] [] ((Ssig (Nid 0) (Enat 4));;(Ssig (Nid 0) (Enat 4))))
-            // (Cps 6 [] [] (Ssig (Nid 0) (Enat 4)))
-            // (Cps 7 [] [] (Ssig (Nid 0) (Enat 4)))).
+  design_ (entid    : ident)      (** Entity id *)
+          (archid   : ident)      (** Architecture id *)
+          (gens     : list gdecl) (** Generic constant list *)
+          (ports    : list pdecl) (** Port list *)
+          (adecls   : list adecl) (** Architecture declarative part *)
+          (behavior : cs).        (** Concurrent statement part *)
