hvhdl/Environment.v
@@ -1,0 +1,64 @@
+(** Module defining the components of the simulation environment.  *)
+
+Require Import Coqlib.
+Require Import GlobalTypes.
+Require Import AbstractSyntax.
+Require Import HilecopDefinitions.
+Require Import SemanticalDomains.
+
+(** Defines the design environment describing H-VHDL design instances
+    in the semantical world. The design environment maps identifiers
+    of a certain category of constructs (e.g, constant identifiers) to
+    their declaration information (e.g, type and value for
+    constants). *)
+
+(* Needed because [SemanticalObject] as a recurvise definition that
+   does not respect the strict positivity requirement.
+   
+   However, I am almost sure that it is not dangerous to do so. *)
+
+Local Unset Positivity Checking.
+
+(** Type of semantical objects that populate the design
+    environment. *)
+                                                     
+Inductive SemanticalObject : Type :=
+| Generic (t : type) (v : value)
+| Constant (t : type) (v : value)
+| Input (t : type)
+| Output (t : type)
+| Declared (t : type)
+| Process (lenv : IdMap (type * value))
+| Component (denv : IdMap SemanticalObject) (behavior : cs).
+
+(** Macro definition for the design environment type. 
+    Mapping from identifiers to 
+ *)
+
+Definition DEnv := IdMap SemanticalObject.
+
+(** Defines an empty design environment. *)
+
+Definition EmptyDEnv   := NatMap.empty SemanticalObject.
+
+(** Defines the structure of design state. *)
+
+Inductive DState : Type :=
+  MkDState {
+      denv      : DEnv;
+      sigstore  : IdMap value;
+      compstore : IdMap DState;
+      events    : IdSet;
+    }.
+
+(** Defines an empty design state. *)
+
+Definition EmptyDState := MkDState EmptyDEnv
+                                   (NatMap.empty value)
+                                   (NatMap.empty DState)
+                                   (NatSet.empty).
+
+(** Definition of the [dom] function that yields a list of identifiers
+    corresponding to the definition domain of an IdMap. *)
+
+Definition dom {A : Type} (f : IdMap A) : list ident := fs (NatMap.elements f).
