hvhdl/ExpressionEvaluation.v
@@ -1,0 +1,38 @@
+(** Module that implement the relation evaluating H-VHDL
+    expressions. *)
+
+Require Import Coqlib.
+Require Import GlobalTypes.
+Require Import AbstractSyntax.
+Require Import Environment.
+Require Import SemanticalDomains.
+
+(** Defines the expression evaluation relation. 
+    
+    The environment is composed of:
+    - [denv], the design environment.
+    - [dstate], the design state.
+    - [lenv], a local environment (process environment).
+    
+ *)
+
+Inductive vexpr (denv : DEnv) (dstate : DState) (lenv : IdMap (type * value)) :
+  expr -> option value -> Prop :=
+
+(** Evaluates nat constant. *) 
+| VExprNat (n : nat) : n <= NATMAX -> vexpr denv dstate lenv (e_nat n) (Some (Vnat n))
+
+(** Evaluates bool constant. *)
+| VExprBool (b : bool) : vexpr denv dstate lenv (e_bool b) (Some (Vbool b))
+
+(** Evaluates arc_t constant. *)
+| VExprArcT (a : arc_t) : vexpr denv dstate lenv (e_arc a) (Some (Varc a))
+
+(** Evaluates arc_t constant. *)
+| VExprTransT (t : transition_t) : vexpr denv dstate lenv (e_trans t) (Some (Vtransition t)).
+                                
+(** Evaluates aggregate expression. *)
+| VExprAggreg (le : list expr) (lv : list value) :
+    (forall (e : expr), In e le -> vexpr denv dstate lenv e (Some v) /\ In v lv) ->
+    length le = length lv
+      
