hvhdl/GlobalTypes.v
@@ -18,4 +18,19 @@ Definition IdMap (A : Type) := NatMap.t A.
 
 Definition IdSet := NatSet.t.
 
+(** Defines the type of Petri net arcs. *)
 
+Inductive arc_t : Type := basic | test | inhibitor.
+
+(** Defines the type of Petri net transitions. *)
+
+Inductive transition_t : Type := not_temporal | temporal_a_b |
+                                 temporal_a_a | temporal_a_inf.
+
+(** Defines the maximum value taken by a natural number
+    in H-VHDL.
+
+    For now, NATMAX equals 2^31 - 1 (max. value on 32 bits).
+ *)
+
+Definition NATMAX := 2147483647.
