hvhdl/IsOfType.v
@@ -1,0 +1,29 @@
+(** Module that defines the typing relation, i.e the relation that
+    checks that a value belongs to a certain type.
+
+    Particularly for [nat] and [array], a value belongs to these type
+    if it satisfies the range or index constraint.  *)
+
+Require Import Coqlib.
+Require Import GlobalTypes.
+Require Import SemanticalDomains.
+
+(** Defines the typing relation [is_of_type]. *)
+
+Inductive is_of_type : value -> type -> Prop :=
+| IsBool : forall (b : bool), is_of_type (Vbool b) Tbool
+| IsArcT : forall (a : arc_t), is_of_type (Varc a) Tarc_t
+| IsTransitionT : forall (t : transition_t), is_of_type (Vtransition t) Ttransition_t
+
+(** Value n must satisfy the index constraint, i.e n ∈ [l,u]. *)
+| IsNat : forall (n l u : nat), l <= n <= u -> is_of_type (Vnat n) (Tnat l u)
+
+(** All elements of the value list [lv] must be of type [t],
+    and the length of [lv] must satisfy the index constraint.
+ *)
+| IsArrayOfT :
+    forall (lv : list value) (t : type) (l u : nat),
+      (forall (v : value), In v lv -> is_of_type v t) ->
+      length lv = u - l + 1 ->
+      is_of_type (Vlist lv) (Tarray t l u).
+      
