hvhdl/SemanticalDomains.v
@@ -1,10 +1,8 @@
-(** Module defining the type of identifiers and values that are common
-    to the syntax and the semantics of H-VHDL.  *)
+(** Module defining the semantics domains used in H-VHDL semantics. *)
 
 Require Import Coqlib.
 Require Import GlobalTypes.
 Require Import AbstractSyntax.
-Require Import HilecopDefinitions.
 
 (** Defines the type of values used in the 
     semantical world.
@@ -12,108 +10,25 @@ Require Import HilecopDefinitions.
     A value is either:
     - a boolean
     - a natural number
+    - an element of arc_t
+    - an element of transition_t
     - a list of values. *)
 
 Inductive value : Type :=
 | Vbool : bool -> value
 | Vnat : nat -> value
+| Varc : arc_t -> value
+| Vtransition : transition_t -> value
 | Vlist : list value -> value.
 
 (** Defines the type of types used in the
     semantical world. *)
 
 Inductive type : Type :=
-| T (tid : typeid)                (** Type id *)
-    (constr : option (nat * nat)) (** Constraint is either a couple of
-                                      nat, or null (i.e, None here) *)
-with typeid : Type :=
-| Tid (id : ident)              (** User-defined type id. *)
-| Tnat                          (** Natural *)
-| Tbool                         (** Boolean *)
-| Tarray (t : type).            (** Array of a certain type. *)
+| Tbool                                 (** Boolean *)
+| Tnat (l : nat) (u : nat)              (** Constrained natural. *)
+| Tarray (t : type) (l : nat) (u : nat) (** Fixed-size array. *)
+| Tarc_t                                (** arc_t type. *)
+| Ttransition_t.                        (** transition_t type. *)
 
-(** Defines the type of type definitions used in
-    the semantical world.
- *)
 
-Inductive typedef : Type :=
-| Tdef_t (t : type)              (** Type definition as an alias to
-                                     another type. *)
-| Tdef_enum (lme : ident)
-            (enum : list ident). (** Type definition as a non-empty definition 
-                                     of identifiers. *)
-
-(** Defines the design structure describing 
-    H-VHDL design instances in the semantical world. *)
-
-(* Needed because design_struct as a recurvise definition that does
-   not respect the strict positivity requirement.  
-   
-   However, I am not sure that it is too dangerous to do so. *)
-
-Local Unset Positivity Checking.
-
-Inductive design_struct : Type :=
-  mk_design {
-      Gens     : IdMap (type * value * value);
-      Ins      : IdMap type;
-      Outs     : IdMap type;
-      Sigs     : IdMap type;
-      Consts   : IdMap (type * value);
-      Ps       : IdMap (IdMap (type * value));
-      Comps    : IdMap design_struct;
-      Types    : IdMap typedef;
-      Behavior : cs;
-    }.
-
-(** Defines empty map for all fields of the design_struct. *)
-
-Definition empty_gens := NatMap.empty (type * value * value).
-Definition empty_ins := NatMap.empty type.
-Definition empty_outs := NatMap.empty type.
-Definition empty_sigs := NatMap.empty type.
-Definition empty_consts := NatMap.empty (type * value).
-Definition empty_localenv := NatMap.empty (IdMap (type * value)).
-Definition empty_comps := NatMap.empty design_struct.
-Definition empty_types := NatMap.empty typedef.
-
-(** Defines an empty design_struct instance.
-
-    The type of empty_design is cs -> design_struct because the
-    Behavior field as no value yet.  *)
-
-Definition empty_design : cs -> design_struct :=
-  mk_design
-    empty_gens empty_ins empty_outs empty_sigs empty_consts
-    empty_localenv empty_comps empty_types.
-
-(** Defines the structure of design state. *)
-
-Inductive design_state : Type :=
-  mk_design_state {
-      sigstore  : IdMap value;
-      compstore : IdMap design_state;
-      events    : IdSet;
-    }.
-
-(** Definition of the [dom] function that yields a list of identifiers
-    corresponding to the definition domain of an IdMap. *)
-
-Definition dom {A : Type} (f : IdMap A) : list ident := fs (NatMap.elements f).
-
-(** Definition of the [enum] function that yields a list of
-    identifiers corresponding to all identifiers contained in the data
-    part of map [f], which is of type [IdMap typedef]. *)
-
-Fixpoint enum_aux (ltypedef : list typedef) {struct ltypedef} : list ident :=
-  match ltypedef with
-  | nil => nil
-  | cons t tl =>
-    match t with
-    | Tdef_enum hd e => [hd] ++ e ++ enum_aux tl
-    | _ => enum_aux tl
-    end
-  end.
-
-Definition enum (f : IdMap typedef) : list ident :=
-  enum_aux (snd (split (NatMap.elements f))).
