hvhdl/StaticExpressions.v
@@ -1,0 +1,49 @@
+(** Predicates for static expression qualification. 
+    
+    A static expression is either locally or globally static.
+ *)
+
+Require Import Coqlib.
+Require Import GlobalTypes.
+Require Import AbstractSyntax.
+Require Import Environment.
+Require Import SemanticalDomains.
+
+Include NatMap.
+
+(** Defines the inductive predicate [is_lstatic_expr] stating that an
+    expression is locally static, i.e it is:
+    
+    - composed of operators and operands of a scalar type (i.e,
+      natural, boolean, arc_t or transition_t).  
+    - a literal of a scalar type.
+ *)
+
+Inductive is_lstatic_expr : expr -> Prop :=
+| IsLStaticNat (n : nat) : is_lstatic_expr (e_nat n)
+| IsLStaticBool (b : bool) : is_lstatic_expr (e_bool b)
+| IsLStaticArc (a : arc_t) : is_lstatic_expr (e_arc a)
+| IsLStaticTransition (t : transition_t) : is_lstatic_expr (e_trans t)
+| IsLStaticNot (e : expr) : is_lstatic_expr e -> is_lstatic_expr (e_not e)
+| IsLStaticBinOp (e e' : expr) (bop : binop) :
+    is_lstatic_expr e -> is_lstatic_expr e' -> is_lstatic_expr (e_binop bop e e').
+
+(** Defines the inductive predicate [is_gstatic_expr] stating that an
+    expression is globally static, i.e it is:
+    
+    - a generic constant.
+    - a constant.
+    - an array aggregate composed of globally static expressions.
+    - a locally static expression.
+ *)
+
+Inductive is_gstatic_expr (env : DEnv) : expr -> Prop :=
+| IsGStaticLStatic (e : expr) : is_lstatic_expr e -> is_gstatic_expr env e
+| IsGStaticGeneric (id : ident) :
+    forall (t : type) (v : value), MapsTo id (Generic t v) env -> is_gstatic_expr env (e_name (n_id id))
+| IsGStaticConstant (id : ident) :
+    forall (t : type) (v : value), MapsTo id (Constant t v) env -> is_gstatic_expr env (e_name (n_id id))
+| IsGStaticAggreg (l : list expr) :
+    (forall (e : expr), List.In e l -> is_gstatic_expr env e) ->
+    is_gstatic_expr env (e_aggreg l).
+    
