hvhdl/TypeElaboration.v
@@ -1,0 +1,5 @@
+Require Import SemanticalDomains.
+Require Import AbstractSyntax.
+
+Inductive etype : tind -> type -> Prop :=
+| etype_nat : etype Tind_natural (Tbase Tnat).
