utils/Arrays.v
@@ -1,0 +1,31 @@
+(** Module that defines the array structure.
+
+    Arrays are a main data structure of the H-VHDL semantics.  *)
+
+Require Import Vector.
+
+(** Defines the interface of arrays with indexes of the [nat] type. *)
+
+Module Type ARRAY.
+
+  (* Type of the array of [elt] of size [nat]. *)
+  Parameter array : nat -> Type -> Type.
+  
+  (* Array creation. *)
+  Parameter create : forall (n : nat) (A : Type), A -> array n A.
+
+  (* Access to an array element. *)
+  Parameter read : forall (n : nat) (A : Type), array n A -> nat -> A.
+
+  (* Store an element in the array. *)
+  Parameter write : forall (n : nat) (A : Type), A -> nat -> array n A -> array n A.
+
+End ARRAY.
+
+(** Implementation of the ARRAY interface with lists. *)
+
+Module Array : ARRAY.
+
+  Definition array (size : nat) (A : Type) := Vector.t A size.
+  
+End Array.
